new source

source.v
@@ -6,360 +6,143 @@ From istari Require Import Sigma Tactics Equality Ordinal Page.
 
 Import List.ListNotations.
 
+Inductive term: Set :=
+| var : nat -> term
+| nattp_m : term
+| z_m : term
+| succ_m : term -> term
+| arrow_m : term -> term -> term
+| lam_m : term -> term
+| app_m : term -> term -> term
+| comp_m : term -> term
+| ret_m : term -> term
+| bind_m : term -> term -> term
+| reftp_m: term -> term
+| ref_m : term -> term
+| deref_m: term -> term
+| assign_m: term -> term
+| triv_m: term
+| unittp_m: term.
 
-Section Object.
-
-
-  Variable object : Type.
-
-Inductive operator : list nat -> Type :=
-| oper_nat: operator nil
-| oper_z: operator nil
-|oper_succ_m: operator [0]
-
-| oper_arrow_m       : operator [0; 0]
-| oper_lam_m         : operator [1]
-| oper_app_m         : operator [0; 0]
-
-| oper_comp_m: operator [0]
-| oper_ret_m: operator [0]
-| oper_bind_m : operator [0; 1] (*bind x = e1 in e2*)
-
-| oper_reftp_m: operator [0]
-| oper_ref_m: operator [0]
-| oper_deref_m: operator [0]
-| oper_assign_m: operator [0; 0] (*R := v*)
-
-| oper_triv_m        : operator nil
-| oper_unittp_m      : operator nil
-| oper_obj: object -> operator nil
-.
+Definition context := list term.
 
 
-Inductive term : Type :=
-| var : nat -> term (*cant have type variables in this language*)
-| oper : forall a, operator a -> row a -> term
+Fixpoint traverse (S:Set) (enter : S -> S) (resolve : S -> nat -> term) (s : S) (t : term) {struct t} : term :=
+  match t with
+   | var i => resolve s i
+   | nattp_m => nattp_m
+   | z_m => z_m
+   | succ_m t1 => succ_m (traverse S enter resolve s t1)
+   | arrow_m t1 t2 => arrow_m (traverse S enter resolve s t1) (traverse S enter resolve s t2)
+   | lam_m t1 => lam_m (traverse S enter resolve (enter s) t1)
+   | app_m t1 t2 => app_m (traverse S enter resolve s t1) (traverse S enter resolve s t2)
+   | comp_m t1 => comp_m (traverse S enter resolve s t1)
+   | ret_m t1 => ret_m (traverse S enter resolve s t1)
+   | bind_m t1 t2 => bind_m (traverse S enter resolve s t1) (traverse S enter resolve (enter s) t2)
+   | reftp_m t1 => reftp_m (traverse S enter resolve s t1)
+   | ref_m t1 => ref_m (traverse S enter resolve s t1)
+   | deref_m t1 => deref_m (traverse S enter resolve s t1)
+   | assign_m t1 => assign_m (traverse S enter resolve s t1)
+   | triv_m => triv_m
+   | unittp_m => unittp_m end.
 
-with row : list nat -> Type :=
-| rw_nil : row nil
-| rw_cons : forall i a, term -> row a -> row (i :: a)
-.
-
-Scheme term_mut_ind := Induction for term Sort Prop
-with   row_mut_ind := Induction for row Sort Prop.
-Combined Scheme syntax_ind from term_mut_ind, row_mut_ind.
-
-Scheme term_mut_rect := Induction for term Sort Type
-with   row_mut_rect := Induction for row Sort Type.
-
-
-Lemma row_nil_invert : forall (r : row nil), r = rw_nil.
-Proof.
-intros r.
-apply eq_dep_impl_eq_snd.
-set (a := nil) in r |- * at 1.
-assert (a = nil) as Heq by reflexivity.
-clearbody a.
-revert Heq.
-cases r; auto.
-intros; discriminate.
-Qed.
-
-
-Lemma row_cons_invert :
-  forall i a (r : row (cons i a)),
-    exists m (s : row a),
-      r = rw_cons i a m s.
-Proof.
-intros i a r.
-cut (exists m s, eq_dep _ row (cons i a) r (cons i a) (rw_cons i a m s)).
-  {
-  intros (m & s & Heq).
-  exists m, s.
-  exact (eq_dep_impl_eq_snd _#5 Heq).
-  }
-set (b := cons i a) in r |- * at 1.
-assert (b = cons i a) as Heq by reflexivity.
-clearbody b.
-revert Heq.
-cases r; try (intros; discriminate).
-intros i' a' m r Heq.
-injection Heq.
-intros -> ->.
-exists m, r.
-apply eq_dep_refl.
-Qed.
+Ltac prove_traverse_parametric ind :=
+intros S S' R enter enter' resolve resolve' s s' t Henter Hresolve Hs;
+generalize dependent s';
+generalize dependent s;
+induction t using ind; intros s s' Hs;
+[apply Hresolve; apply Hs | ..];  (* deal with first goal (var) *)
+simpl;
+try reflexivity;  (* dispense with trivial goals *)
+f_equal;
+(* find and apply IH *)
+try
+  ((match goal with
+    | IH : (forall (s : S) (s' : S'), _ -> _ = ?f _ ?t)
+      |- _ = ?g _ ?t
+      => apply IH
+    end);
+   repeat (apply Henter);
+   apply Hs).
 
 
-Lemma row_invert_auto :
-  forall a (r : row a),
-    list_rect (fun a => (row a -> Prop) -> Prop)
-      (fun P => P rw_nil)
-      (fun i a IH P =>
-         exists m,
-           IH (fun r => P (rw_cons i a m r)))
-      a
-      (eq r).
-Proof.
-intros a.
-induct a.
-
-(* nil *)
-{
-intro r.
-cbn.
-apply row_nil_invert.
-}
-
-(* cons *)
-{
-intros i a IH rr.
-cbn.
-so (row_cons_invert _ _ rr) as (m & r & ->).
-exists m.
-force_exact (IH r).
-f_equal.
-fextensionality 1.
-intro r'.
-pextensionality.
-  {
-  intros <-; auto.
-  }
-
-  {
-  intros Heq.
-  injection Heq.
-  intro H.
-  injectionT H.
-  auto.
-  }
-}
-Qed.
+Ltac prove_traverse_id ind :=
+intros S R enter resolve s t Henter Hresolve Hs;
+generalize dependent s;
+induction t using ind; intros s Hs;
+[apply Hresolve; apply Hs | ..];  (* deal with first goal (var) *)
+simpl;
+try reflexivity;  (* dispense with trivial goals *)
+f_equal;
+(* find and apply IH *)
+try ((match goal with
+      | IH : (forall (s : S), _ -> _ = ?t)
+        |- _ = ?t
+        => apply IH
+      end);
+     repeat (apply Henter);
+     apply Hs).
 
 
-Inductive hyp : Type :=
-(*| hyp_tpl : hyp x: _type_*)
-hyp_tm  : term -> hyp
-.
+Ltac prove_traverse_compose ind :=
+intros S S' enter enter' resolve resolve' s s' t;
+generalize dependent s';
+generalize dependent s;
+induction t using ind; intros s s';
+[simpl; reflexivity | ..];  (* deal with first goal (var) *)
+simpl;
+try reflexivity;  (* dispense with trivial goals *)
+f_equal;
+(* find and apply IH *)
+try (match goal with
+      | IH : (forall (s : S) (s' : S'), _ = ?f ?t)
+        |- _ = ?g ?t
+        => apply IH
+      end).
 
-
-Definition context := list hyp.
-
-
-Inductive judgement : Type :=
-| deq : (* tm *) term -> term -> (* cn *) term -> judgement
-| typ: term -> judgement
-.
-
-
-
-Fixpoint traverse (resolve : nat -> nat -> term) (i : nat) (m : term) {struct m} : term
-  :=
-  (match m with
-   | var j => resolve i j
-   | oper a t r => oper a t (traverse_row resolve i a r)
-   end)
-
-with traverse_row (resolve : nat -> nat -> term) (i : nat) (a : list nat) (r : row a) {struct r} : row a
-  :=
-  (match r
-   in row a
-   return row a
-   with
-   | rw_nil => rw_nil
-   | rw_cons j a m r => rw_cons j a (traverse resolve (j+i) m) (traverse_row resolve i a r)
-   end)
-.
 
 
 Lemma traverse_var :
-  forall resolve i j,
-    traverse resolve i (var j) = resolve i j.
+  forall S enter resolve s i,
+    traverse S enter resolve s (var i) = resolve s i.
 Proof.
 auto.
-Qed.
-
-
-Lemma traverse_oper :
-  forall resolve i a t r,
-    traverse resolve i (oper a t r)
-    =
-    oper a t (traverse_row resolve i a r).
-Proof.
-intros; reflexivity.
-Qed.
-
-
-Lemma traverse_row_cons :
-  forall resolve i j a m r,
-    traverse_row resolve i (cons j a) (rw_cons j a m r)
-    =
-    rw_cons j a
-      (traverse resolve (j+i) m)
-      (traverse_row resolve i a r).
-Proof.
-intros; reflexivity.
-Qed.
-
-
-Lemma traverse_row_nil :
-  forall resolve i,
-    traverse_row resolve i nil rw_nil = rw_nil.
-Proof.
-intros; reflexivity.
 Qed.
 
 
 Lemma traverse_parametric :
-  forall (P : nat -> nat -> Prop) resolve resolve',
-    (forall i i', P i i' -> P (S i) (S i'))
-    -> (forall i i' j, P i i' -> resolve i j = resolve' i' j)
-    -> forall i i' t, P i i' -> traverse resolve i t = traverse resolve' i' t.
-Proof.
-intros P resolve resolve' Pcomp.
-revert resolve resolve'.
-assert (forall j i i', P i i' -> P (j + i) (j + i')) as Hcomp'.
-  intro j.
-  induct j.
-  (* 0 *)
-  intros i i' H.
-  exact H.
-
-  (* S *)
-  intros j IH i i' HP.
-  simpl.
-  auto; done.
-intros resolve resolve' Hres i i' t.
-revert t i i'.
-apply
-  (term_mut_ind
-     (fun m => forall i i', P i i' -> traverse resolve i m = traverse resolve' i' m)
-     (fun a r => forall i i', P i i' -> traverse_row resolve i a r = traverse_row resolve' i' a r));
-try (intros; simpl; eauto; f_equal; eauto; done).
+  forall (S:Set) (S':Set) (R : S -> S' -> Prop) enter enter' resolve resolve' s s' t,
+    (forall s s', R s s' -> R (enter s) (enter' s'))
+    -> (forall s s' i, R s s' -> resolve s i = resolve' s' i)
+    -> R s s'
+    -> traverse S enter resolve s t = traverse S' enter' resolve' s' t.
+Proof. 
+prove_traverse_parametric term_ind.
 Qed.
 
 
 Lemma traverse_id :
-  forall resolve,
-    (forall i j, resolve i j = var j)
-    -> forall i t, traverse resolve i t = t.
+  forall (S:Set) (R : S -> Prop) enter resolve s t,
+    (forall s, R s -> R (enter s))
+    -> (forall s i, R s -> resolve s i = var i)
+    -> R s
+    -> traverse S enter resolve s t = t.
 Proof.
-intros resolve Hres i m.
-revert m i.
-apply
-  (term_mut_ind
-     (fun m => forall i, traverse resolve i m = m)
-     (fun a r => forall i, traverse_row resolve i a r = r));
-intros; simpl; f_equal; eauto.
+prove_traverse_id term_ind.
 Qed.
 
 
 Lemma traverse_compose :
-  forall resolve resolve' i t,
-    traverse resolve i (traverse resolve' i t)
-    = traverse
-      (fun i' j => traverse resolve i' (resolve' i' j))
-      i t.
+  forall (S:Set) (S':Set) enter enter' resolve resolve' s s' t,
+    traverse S enter resolve s (traverse S' enter' resolve' s' t)
+    = traverse (S * S')
+      (fun p => let (s, s') := p in (enter s, enter' s'))
+      (fun p i => let (s, s') := p in traverse S enter resolve s (resolve' s' i))
+      (s, s') t.
 Proof.
-intros resolve resolve' i m.
-revert m i.
-apply
-  (term_mut_ind
-     (fun m =>
-        forall i, 
-          traverse resolve i (traverse resolve' i m)
-          = traverse (fun i' j => traverse resolve i' (resolve' i' j)) i m)
-     (fun a r =>
-        forall i, 
-          traverse_row resolve i a (traverse_row resolve' i a r)
-          = traverse_row (fun i' j => traverse resolve i' (resolve' i' j)) i a r));
-intros; simpl; f_equal; eauto.
+prove_traverse_compose term_ind.
 Qed.
 
 
-
-Inductive Forallr (P : term -> Type) : forall a, row a -> Type :=
-| Forallr_nil
-    : Forallr P nil rw_nil
-
-| Forallr_cons {i a m r}
-    : P m
-      -> Forallr P a r
-      -> Forallr P (cons i a) (rw_cons i a m r)
-.
-
-
-Lemma term_row_rect :
-  forall (P : term -> Type),
-    (forall i, P (var i))
-    -> (forall a t r, Forallr P a r -> P (oper a t r))
-    -> forall m, P m.
-Proof.
-intros P H1 H2 m.
-apply (term_mut_rect P (Forallr P)); eauto using Forallr.
-Qed.
-
-
-Lemma oper_injection :
-  forall a t t' r r',
-    oper a t r = oper a t' r'
-    -> t = t' /\ r = r'.
-Proof.
-intros a t t' r r' Heq.
-injection Heq.
-intros Heqr Heqt.
-destruct (eq_dep_impl_eq _#6 (EqdepFacts.eq_sigT_eq_dep _#6 Heqt)) as (h & Heqt').
-substrefl h.
-cbn in Heqt'.
-destruct (eq_dep_impl_eq _#6 (EqdepFacts.eq_sigT_eq_dep _#6 Heqr)) as (h & Heqr').
-substrefl h.
-cbn in Heqr'.
-auto.
-Qed.
-
-
-Lemma rw_cons_injection :
-  forall j a m m' r r',
-    rw_cons j a m r = rw_cons j a m' r'
-    -> m = m' /\ r = r'.
-Proof.
-intros j a m m' r r' Heq.
-injection Heq.
-intros Heq' Heqm.
-destruct (eq_dep_impl_eq _#6 (EqdepFacts.eq_sigT_eq_dep _#6 Heq')) as (h & Heq'').
-substrefl h.
-cbn in Heq''.
-auto.
-Qed.
-End Object.
-
-Arguments var {object}.
-Arguments oper {object}.
-Arguments rw_nil {object}.
-Arguments rw_cons {object}.
-
-Arguments hyp {object}.
-Arguments context {object}.
-Arguments judgement {object}.
-
-Definition nattp_m {obj}: @term obj := oper _ (oper_nat _) rw_nil.
-Definition z_m {obj}: @term obj := oper _ (oper_z _) rw_nil.
-Definition succ_m {obj} M: @term obj := oper _ (oper_succ_m _) (rw_cons _ _ M rw_nil).
-Definition arrow_m {obj} m1 m2 : @term obj := oper _ (oper_arrow_m _) (rw_cons _ _ m1 (rw_cons _ _ m2 rw_nil)).
-Definition lam_m {obj} m             : @term obj := oper _ (oper_lam_m _) (rw_cons _ _ m rw_nil).
-Definition app_m {obj} m1 m2         : @term obj := oper _ (oper_app_m _) (rw_cons _ _ m1 (rw_cons _ _ m2 rw_nil)).
-
-Definition comp_m {obj} T : @term obj := oper _ (oper_comp_m _) (rw_cons _ _ T rw_nil).
-Definition ret_m {obj} M : @term obj := oper _ (oper_ret_m _) (rw_cons _ _ M rw_nil).
-Definition bind_m {obj} m1 m2 : @term obj := oper _ (oper_bind_m _) (rw_cons _ _ m1 (rw_cons _ _ m2 rw_nil)).
-Definition reftp_m {obj} T : @term obj := oper _ (oper_reftp_m _) (rw_cons _ _ T rw_nil).
-Definition ref_m {obj} M : @term obj := oper _ (oper_ref_m _) (rw_cons _ _ M rw_nil).
-Definition deref_m {obj} M : @term obj := oper _ (oper_deref_m _) (rw_cons _ _ M rw_nil).
-Definition asgn_m {obj} m1 m2 : @term obj := oper _ (oper_assign_m _) (rw_cons _ _ m1 (rw_cons _ _ m2 rw_nil)).
-
-Definition unittp_m  {obj}     : @term obj := oper _ (oper_unittp_m _) rw_nil.
-Definition triv_m   {obj}    : @term obj := oper _ (oper_triv_m _) rw_nil.
-
-Arguments hyp_tm {object}.
-Arguments deq {object}.
-Arguments typ {object}.
+Definition termx := term.
+Definition varx := var.
